Relations now represented properly.

CompilerWorks.v
@@ -2,29 +2,48 @@ From Coq Require Import Strings.String.
 From Coq Require Import Lists.List.
 Import ListNotations.
 
+(* Transformer: switches b/w dialects, prove rel is involution. *)
+(* Optimization: remove unused tables from FROM/JOIN clauses. *)
+
 Local Open Scope string_scope.
 
-Inductive stmt : Type :=
-| Select (fld: string).
+Inductive jclause : Type :=
+| Join (relation: list (string -> string)) (onlhs : string) (onrhs : string).
 
 Inductive wclause : Type :=
 | WhereEqual (fld : string) (val : string).
 
-(* Transformer: switches b/w dialects, prove rel is involution. *)
-(* Optimization: remove unused tables from FROM/JOIN clauses. *)
+Definition relation : Type := (list string) * list (string -> string).
 
-Definition fruits : list (string -> string) := [
-    fun c => match c with "id"=>"1"|"name"=>"orange"|"price"=>"5"|_=>"" end ;
+Inductive sqlstmt : Type :=
+| Select (flds: list string) (rel: relation)
+| SelectWhere (flds: list string) (rel: relation) (wheres: list wclause).
+
+Definition fruits : relation :=
+  (["id" ; "name" ; "price"] ,
+   [fun c => match c with "id"=>"1"|"name"=>"orange"|"price"=>"5"|_=>"" end ;
     fun c => match c with "id"=>"2"|"name"=>"apple"|"price"=>"9"|_=>"" end ;
     fun c => match c with "id"=>"3"|"name"=>"banana"|"price"=>"5"|_=>"" end ;
-    fun c => match c with "id"=>"4"|"name"=>"kiwi"|"price"=>"8"|_=>"" end].
+    fun c => match c with "id"=>"4"|"name"=>"kiwi"|"price"=>"8"|_=>"" end]).
 
-Example ex1 : map (fun r => (r "name")) fruits
-               = ["orange" ; "apple" ; "banana" ; "kiwi"].
-Proof. simpl. reflexivity. Qed.
+Definition render (rel : relation) :=
+    let fix render_aux (flds : list string) (rows : list (string -> string)) :=
+      match flds, rows with
+      | fs, r::rs =>
+        (map (fun f => (r f)) fs) :: (render_aux fs rs)
+      | _, _ => []
+      end
+    in (fst rel) :: render_aux (fst rel) (snd rel).
 
-Definition q1 : stmt := (Select "name").
+Example ex1 : render fruits =
+              [["id" ; "name" ; "price"] ;
+               ["1" ; "orange" ; "5"] ;
+               ["2" ; "apple" ; "9"] ;
+               ["3" ; "banana" ; "5"] ;
+               ["4" ; "kiwi" ; "8"]].
+Proof. unfold render. simpl. reflexivity. Qed.
 
+(*
 Fixpoint evalwhere (w : wclause) (rel : list (string -> string)) :=
   match w with
   | WhereEqual wfld wval =>
@@ -35,29 +54,43 @@ Fixpoint evalwhere (w : wclause) (rel : list (string -> string)) :=
     | _ => []
     end
   end.
+ *)
 
-Fixpoint eval (flds : list string) (rel: list (string->string))
-              (wheres : list wclause) :=
-  match wheres with
-  | whd::wtl => eval flds (evalwhere whd rel) wtl
-  | [] => map (fun r => (map (fun f => (r f)) flds)) rel
+Fixpoint evalstmt (stmt : sqlstmt) : relation :=
+  match stmt with
+  | Select fields rel =>
+    let fix select_fields (flds : list string) (row : (string -> string))
+                          : (string -> string) :=
+      match flds with
+      | f::fs => (fun c => if (string_dec c f)
+                          then (row c) else ((select_fields fs) row) c)
+      | [] => (fun _ => "")
+      end
+    in 
+    (fields, (map (select_fields fields) (snd rel)))
+  | SelectWhere flds rel wclauses => rel
+    (* | whd::wtl => eval flds (evalwhere whd rel) wtl *)
   end.
 
-Example ex2 : (eval ["name"] fruits [])
-              = [["orange"] ; ["apple"] ; ["banana"] ; ["kiwi"] ].
+Example ex2 : (render (evalstmt (Select ["name"] fruits)))
+              = [["name"] ; ["orange"] ; ["apple"] ; ["banana"] ; ["kiwi"] ].
+Proof. unfold render. simpl. reflexivity. Qed. 
+
+Example ex3 : (render (evalstmt (Select ["id";"name"] fruits)))
+              = [["id";"name"] ; ["1";"orange"] ; ["2";"apple"] ;
+                   ["3";"banana"] ; ["4";"kiwi"] ].
 Proof. simpl. reflexivity. Qed.
 
-Example ex3 : (eval ["id";"name"] fruits [])
-              = [["1";"orange"] ; ["2";"apple"] ; ["3";"banana"] ; ["4";"kiwi"] ].
-Proof. simpl. reflexivity. Qed.
+Example ex4 : (render (evalstmt (Select ["name" ; "id"] fruits)))
+              = [["name";"id"] ; ["orange";"1"] ; ["apple";"2"] ; ["banana";"3"] ; ["kiwi";"4"] ].
+Proof. unfold render. simpl. reflexivity. Qed.
 
-Example ex4 : (eval ["name";"id"] fruits [])
-              = [["orange";"1"] ; ["apple";"2"] ; ["banana";"3"] ; ["kiwi";"4"] ].
-Proof. simpl. reflexivity. Qed.
-
-Example ex5 : (eval ["id";"name"] fruits [(WhereEqual "name" "kiwi")])
+(*
+Example ex5 : (render (evalstmt (SelectWhere ["id";"name"] fruits [(WhereEqual "name" "kiwi")])))
               = [ ["4";"kiwi"] ].
-Proof. simpl. reflexivity. Qed.
+Proof. unfold render; simpl.
+
+       reflexivity. Qed.
 
 Example ex6 : (eval ["name"] fruits [(WhereEqual "price" "5")])
               = [ ["orange"] ; ["banana"]].
@@ -66,4 +99,32 @@ Proof. simpl. reflexivity. Qed.
 Example ex7 : (eval ["name"] fruits [(WhereEqual "price" "5");(WhereEqual "id" "3")])
               = [ ["banana"]].
 Proof. simpl. reflexivity. Qed.
+ *)
 
+Example ex6_subquery : (render (evalstmt (Select ["name"]
+                                 (evalstmt (Select ["price";"name"] fruits)))))
+              = [["name"] ; ["orange"] ; ["apple"] ; ["banana"] ; ["kiwi"] ].
+Proof. unfold render. simpl. reflexivity. Qed.
+
+Definition stores : list (string -> string) := [
+    fun c => match c with "sid"=>"1"|"sname"=>"La Tienda"|"sfruit"=>"4"|_=>"" end ;
+    fun c => match c with "sid"=>"2"|"sname"=>"Duka 88"|"sfruit"=>"1"|_=>"" end].
+
+(* TODO: Define a join evaluator that can combine two relations. I envision
+   this is a destructuring of each (string -> string) such that the join
+   column is deduplicated and the entire record itself is only present if
+   the value in the left relation matches that of the right. The important part
+   is that the evaluator shouldn't return lists of strings, it should return
+   proper relations. A separate function (i.e., "render") should "evaluate" the
+   relation itself into actual lists so that we can write proofs about it.
+*)
+Fixpoint eval2 (flds : list string) (rel: list (string->string))
+               (join : jclause) (wheres : list wclause) :=
+  match wheres with
+  | whd::wtl => eval flds (evalwhere whd rel) wtl
+  | [] => map (fun r => (map (fun f => (r f)) flds)) rel
+  end.
+
+Example exj1 : (eval2 ["sname" ; "name"] stores (Join fruits "sfruit" "id") [])
+               = [["orange"] ; ["apple"] ; ["banana"] ; ["kiwi"] ].
+Proof. simpl. reflexivity. Qed.
